rustfrontend/Rustlightown.v
@@ -389,7 +389,7 @@ Fixpoint place_dominator (p: place) : option place :=
   | Pfield p' _ _ => place_dominator p'
   | Pdowncast p' _ _ => Some p'
   | Plocal _ _ => None
-  | Pparenthesize _ _ _ _ => None
+  | Pparenthesize _ _ _ => None
   | ParrayIndex p' _ _ => Some p'
   end.
 
@@ -401,7 +401,7 @@ Fixpoint place_dominators (p: place) : list place :=
       let po := valid_owner p' in
       po :: place_dominators po
   | Plocal _ _ => nil
-  | Pparenthesize _ _ _ _ => nil
+  | Pparenthesize _ _ _ => nil
   | ParrayIndex p' _ _ => place_dominators p'
   end.
 
