extraction/extraction.v
@@ -135,7 +135,9 @@ Extract Constant Compiler.print_Rustlight => "PrintRustlight.print_if".
 (* Rust Compiler *)
 Extract Constant Clightgen.create_union_idents => "Dropglue.create_union_idents".
 Extract Constant Clightgen.malloc_id => "Dropglue.malloc_id".
+Extract Constant Clight2Rustlight.malloc_id => "Dropglue.malloc_id".
 Extract Constant Clightgen.free_id => "Dropglue.free_id".
+Extract Constant Clight2Rustlight.free_id => "Dropglue.free_id".
 Extract Constant Clightgen.param_id => "Dropglue.param_id".
 Extract Constant Clightgen.fresh_atom => "Camlcoq.fresh_atom".
 Extract Constant ElaborateDrop.fresh_atom => "Camlcoq.fresh_atom".
